Finished the Cexec proofs again, and filled in external functions

cfrontend/EF.ml
@@ -1,0 +1,80 @@
+open Ctypes
+
+let extern_functions = [
+        (((AST.EF_malloc,
+        Tcons(Tlong(Unsigned, noattr),Tnil)),
+        Tpointer(Tvoid,noattr)),
+        AST.cc_default);
+        
+        (((AST.EF_free,
+        Tcons(Tpointer(Tvoid, noattr),Tnil)),
+        Tvoid),
+        AST.cc_default);
+
+        (((AST.EF_external(Camlcoq.coqstring_of_camlstring "printf",
+                                {AST.sig_args = [AST.Tlong];
+                                 AST.sig_res = AST.Tret(AST.Tint);
+                                 AST.sig_cc = AST.cc_default;}),
+        Tcons(Tint(I8,Signed,noattr),Tnil)),
+        Tint(I32,Signed,noattr)),
+        AST.cc_default);
+
+        (((AST.EF_external(Camlcoq.coqstring_of_camlstring "fgets",
+                                {AST.sig_args = [AST.Tlong; AST.Tint];
+                                 AST.sig_res = AST.Tret(AST.Tlong);
+                                 AST.sig_cc = AST.cc_default;}),
+        Tcons(Tlong(Signed,noattr),Tcons(Tint(I8,Signed,noattr),Tnil))),
+        Tlong(Signed,noattr)),
+        AST.cc_default);
+]
+
+(** Add declarations for the helper functions
+    (for varargs and for int64 arithmetic) *)
+
+(*let helper_functions () = [
+    "__compcert_va_int32",
+        Tint(I32, Unsigned, noattr),
+        [Tpointer(Tvoid, noattr)];
+    "__compcert_va_int64",
+        Tlong(Unsigned, noattr),
+        [Tpointer(Tvoid, noattr)];
+    "__compcert_va_float64",
+        Tfloat(F64, noattr),
+        [Tpointer(Tvoid, noattr)];
+    "__compcert_va_composite",
+        Tpointer(Tvoid, noattr),
+        [Tpointer(Tvoid, noattr); convertIkind (Cutil.size_t_ikind()) noattr];
+    "__compcert_i64_dtos",
+        Tlong(Signed, noattr),
+        [Tfloat(F64, noattr)];
+    "__compcert_i64_dtou",
+        Tlong(Unsigned, noattr),
+        [Tfloat(F64, noattr)];
+    "__compcert_i64_stod",
+        Tfloat(F64, noattr),
+        [Tlong(Signed, noattr)];
+    "__compcert_i64_utod",
+        Tfloat(F64, noattr),
+        [Tlong(Unsigned, noattr)];
+    "__compcert_i64_stof",
+        Tfloat(F32, noattr),
+        [Tlong(Signed, noattr)];
+    "__compcert_i64_utof",
+        Tfloat(F32, noattr),
+        [Tlong(Unsigned, noattr)];
+    "__compcert_i64_sdiv",
+        Tlong(Signed, noattr),
+        [Tlong(Signed, noattr); Tlong(Signed, noattr)];
+    "__compcert_i64_udiv",
+        Tlong(Unsigned, noattr),
+        [Tlong(Unsigned, noattr); Tlong(Unsigned, noattr)];
+    "__compcert_i64_smod",
+        Tlong(Signed, noattr),
+        [Tlong(Signed, noattr); Tlong(Signed, noattr)];
+    "__compcert_i64_umod",
+        Tlong(Unsigned, noattr),
+        [Tlong(Unsigned, noattr); Tlong(Unsigned, noattr)];
+    "__compcert_i64_shl",
+        Tlong(Signed, noattr),
+        [Tlong(Signed, noattr); Tint(I32, Signed, noattr)];
+]*)
